Foundation/Modal/Kripke/Hilbert/S4.lean
@@ -44,7 +44,7 @@ instance finiteComplete : Complete (Hilbert.S4) Kripke.FrameClass.finite_preorde
   replace F_preorder := Set.mem_setOf_eq.mp F_preorder;
   let M : Kripke.Model := ⟨F, V⟩;
   let FM := finestFilterationTransitiveClosureModel M φ.subformulas;
-  apply filteration FM (finestFilterationTransitiveClosureModel.filterOf) (by aesop) |>.mpr;
+  apply filteration FM (finestFilterationTransitiveClosureModel.filterOf) (by subformula) |>.mpr;
   apply hp;
   refine ⟨?_, ?_⟩;
   . apply FilterEqvQuotient.finite;
